add lemmas for (* ubDom *) (* ubRestrict *) (* ubGetCh *) (* ubLeast *) (* ubLen *)  (* ubShift *)

UBundle.thy
@@ -110,18 +110,219 @@ definition ubShift :: "('a \<Rightarrow> 'b) \<Rightarrow> 'a ubundle \<Rightarr
 (****************************************************)
 section\<open>Lemmas\<close>
 (****************************************************)
+(* if ub is a chain then its unlifted functions are also a chain  *)
+lemma rep_chain[simp]: assumes "chain S"
+  shows "chain (\<lambda>n. Rep_ubundle (S n))"
+  by (meson assms below_ubundle_def po_class.chain_def)
 
+(* the lub of a channel in a chain is the same as when apply on each element of the chain  *)
+lemma lub_eval: assumes "chain S"
+  shows "the (Rep_ubundle (\<Squnion>i. S i) c) = (\<Squnion>j. the (Rep_ubundle (S j) c))"
+  by (metis (mono_tags) Abs_ubundle_inverse Rep_ubundle adm_def assms lub_ubundle mem_Collect_eq part_the_lub rep_chain ubWell_adm)
+
+  subsection \<open>ubDom\<close>
 (* ubDom *)
 
-(* ubRestrict *)
-  
+thm ubDom_def
+(*
+definition ubDom :: "'m\<^sup>\<omega> \<rightarrow> channel set" where
+"ubDom \<equiv> \<Lambda> b. dom (Rep_ubundle b)"
+*)
+(* the function udom is continuous *)
+lemma ubDom_cont[simp]: "cont (\<lambda> ub. dom (Rep_ubundle ub))"
+  by (smt Cont.contI2 below_ubundle_def is_ub_thelub monofunI not_below2not_eq part_dom_eq)
+
+(* the dom of ub is the same as the dom of the unlifted ub *)
+lemma ubDom_insert: "ubDom\<cdot>tb = dom (Rep_ubundle tb)"
+  by (simp add: ubDom_def)
+
+(* the dom of the ub is the same as the dom of the lifted function *)
+lemma ubDom_rep_eq: "ubWell ub \<Longrightarrow> ubDom\<cdot>(Abs_ubundle ub) = dom ub"
+  by (simp add: Abs_ubundle_inverse ubDom_insert)
+
+(* if there is a relation between 2 ubs, they two have same dom  *)
+lemma ubDom_below: assumes "ub1 \<sqsubseteq> ub2"
+  shows "ubDom\<cdot>ub1 = ubDom\<cdot>ub2"
+  by (metis assms below_ubundle_def part_dom_eq ubDom_insert)
+
+(* all bundles in a chain have the same dom *)
+lemma ubChain_dom_eq3: assumes "chain S"
+  shows "ubDom\<cdot>(S i) = ubDom\<cdot>(S j)"
+  using assms is_ub_thelub ubDom_below by blast
+                      
+(* all bundles in a chain have the same dom as the lub *)
+lemma ubChain_dom_eq2[simp]: assumes "chain S"
+  shows "ubDom\<cdot>(S i) = ubDom\<cdot>(\<Squnion>j. S j)"
+  by (simp add: assms is_ub_thelub ubDom_below)
+
+(* see ubChain_dom_eq2 *)
+lemma ubDom_lub: assumes "chain Y" and "ubDom\<cdot>(Y i) = cs"
+  shows "ubDom\<cdot>(\<Squnion> i. Y i) = cs"
+  using assms(1) assms(2) by auto
+
+
+  subsection \<open>ubGetCh\<close>
 (* ubGetCh *)
+thm ubGetCh_def
+(* ubGetCh is cont *)
+lemma ubGetCh_cont [simp]: "cont (\<lambda>ub. ((Rep_ubundle ub) \<rightharpoonup> c))"
+  by (smt Prelude.contI2 below_ubundle_def fun_below_iff lub_eq lub_eval monofun_def not_below2not_eq op_the_mono)
 
+(* the element in a channel is the same when it's lifted  *)
+lemma ubGetCh_rep_eq: "ubWell ub \<Longrightarrow> ubGetCh c\<cdot>(Abs_ubundle ub) = ub \<rightharpoonup> c"
+  by (simp add: Abs_ubundle_inverse ubGetCh_def)
+
+(* the element in a channel is the same when unlifted  *)
+lemma ubGetChE: assumes "c \<in> ubDom\<cdot>ub"
+  shows "Some (ubGetCh c\<cdot>ub) = (Rep_ubundle ub) c"
+  by (metis (full_types) Rep_ubundle Rep_ubundle_inverse assms domIff mem_Collect_eq option.exhaust_sel ubGetCh_rep_eq ubDom_insert)
+
+(* the element in a channel of the lub is the same when applying ubGetCh on each ele  *)
+lemma ubGetCh_lub: assumes "chain Y" and "c \<in> ubDom\<cdot>(\<Squnion> i. Y i)"
+  shows "ubGetCh c\<cdot>(\<Squnion>i. Y i) = (\<Squnion>i. ubGetCh c\<cdot>(Y i))"
+  using assms(1) contlub_cfun_arg by auto
+
+(* the element in each channel has the same relation as its bundle  *)
+lemma ubGetCh_below: assumes "x \<sqsubseteq> y"
+  shows "\<forall> c. ubGetCh c\<cdot>x \<sqsubseteq> ubGetCh c\<cdot>y"
+  by (simp add: assms monofun_cfun_arg)
+
+(* the element in a channel is the same when it's unlifted  *)
+lemma ubGetCh_insert: "ubGetCh c\<cdot>ub= (Rep_ubundle ub) \<rightharpoonup> c"
+  by (simp add: ubGetCh_def)
+
+(* induction rule for equal proof of two bundle  *)
+lemma ubGetChI: assumes "ubDom\<cdot>x = ubDom\<cdot>y" and "\<And>c. c\<in>(ubDom\<cdot>x) \<Longrightarrow> ubGetCh c\<cdot>x = ubGetCh c\<cdot>y"
+  shows "x = y"
+  by (metis Rep_ubundle_inject assms(1) assms(2) part_eq ubDom_insert ubGetCh_insert)
+
+(* id function *)
+lemma [simp]: "Abs_ubundle (\<lambda>c. (c \<in> ubDom\<cdot>b)\<leadsto>ubGetCh c\<cdot>b) = b"
+  apply (rule ubGetChI, subst ubDom_rep_eq)
+    apply (smt Rep_ubundle domIff mem_Collect_eq ubGetChE ubWell_def)
+   apply simp
+  by (smt Abs_cfun_inverse2 Abs_ubundle_inverse Rep_ubundle domIff mem_Collect_eq option.sel ubDom_def ubGetChE ubWell_def ubDom_cont)
+
+
+
+subsection \<open>ubLeast\<close>
 (* ubLeast *)
-  
-(* ubLen *) 
 
+  thm ubLeast_def
+
+(* the optionLeast of the optionCpo is well-formed  *)
+lemma ubleast_well: "ubWell (optionLeast cs)"
+  by (simp add: ubWell_def usOkay_bot)
+
+(* our definition of ubLeast is equal optionLeast  *)
+lemma ubLeast_optionLeast_eq: "ubLeast cs = Abs_ubundle(optionLeast cs)"
+  by (simp add: ubLeast_def optionLeast_def)
+  
+(* the dom of ubLeast is the same as the argument of the function  *)
+lemma ubleast_ubDom [simp]: "ubDom\<cdot>(ubLeast cs) = cs"
+  apply (simp add: ubDom_def)
+  by (metis ubLeast_optionLeast_eq optionleast_dom ubDom_insert ubDom_rep_eq ubleast_well)
+
+(* the element in each channel is the bottom element  *)
+lemma ubLeast_getCh[simp]:  assumes "c \<in> cs"
+  shows "ubGetCh c\<cdot>(ubLeast cs) = \<bottom>"
+  by (simp add: assms ubGetCh_rep_eq ubLeast_optionLeast_eq ubleast_well)
+
+(* the ubLeast bundle is the smallest bundle  *)
+lemma tsbleast_below [simp]: assumes "cs = ubDom\<cdot>ub"
+  shows "ubLeast cs \<sqsubseteq> ub"
+  by (metis assms below_ubundle_def minimal part_below ubLeast_getCh ubDom_insert ubGetCh_insert ubleast_ubDom)
+
+(* if ubLeast {} is in an chain, all elements are equal *)
+lemma ubundle_allempty: assumes "chain Y" and "ubLeast {} \<in> range Y"
+  shows "\<And>i. (Y i) = ubLeast {}"
+  by (metis (no_types, lifting) Abs_cfun_inverse2 Rep_ubundle_inverse assms(1) assms(2) empty_iff f_inv_into_f 
+        part_eq ubChain_dom_eq2 ubDom_def ubDom_cont ubleast_ubDom)
+
+
+
+  subsection \<open>ubRestrict\<close>
+(* ubRestrict *)
+thm ubRestrict_def
+
+(* the ubRestrict function returns a well-formed ubundle  *)
+lemma ubRestrict_well [simp]: "ubWell (Rep_ubundle b |` cs)"
+  by (metis (no_types, lifting) Rep_ubundle domIff mem_Collect_eq restrict_in restrict_out ubWell_def)
+
+(* the ubRestrict function is monoton  *)
+lemma ubRestrict_monofun[simp]: "monofun  (\<lambda>b. Rep_ubundle b |` cs)"
+  by (metis (no_types, lifting) below_ubundle_def monofun_def part_restrict_monofun)
+
+(* the ubRestrict function is continuous  part 1*)
+lemma ubRestrict_cont1[simp]: "cont  (\<lambda>b. ((Rep_ubundle b) |` cs))"
+  apply (rule contI2)
+  apply simp
+  by (smt Abs_ubundle_inverse Rep_ubundle adm_def below_option_def domIff fun_below_iff lub_eq lub_fun lub_ubundle mem_Collect_eq 
+      part_dom_lub po_class.chain_def rep_chain restrict_map_def ubChain_dom_eq2 ubWell_adm)
+
+(* the ubRestrict function is continuous *)
+lemma ubRestrict_cont [simp]: "cont (\<lambda>b. Abs_ubundle (Rep_ubundle b |` cs))"
+  by (simp add: cont_Abs_ubundle)
+
+(*   *) 
+lemma ubRestrict_insert : "ubRestrict cs\<cdot>tb = Abs_ubundle (Rep_ubundle tb |` cs)"
+  by (simp add: ubRestrict_def)
+
+(*   *)
+lemma ubRestrict_rep_eq : "ubWell tb \<Longrightarrow> ubRestrict cs\<cdot>(Abs_ubundle tb) = Abs_ubundle (tb |` cs)"
+  by (simp add: Abs_ubundle_inverse ubRestrict_insert)
+
+(* the dom of the bundle after restrict its channel is a subset (or equal) its argument*)
+lemma ubRestrict_dom [simp]: "ubDom\<cdot>(ubRestrict cs\<cdot>tb) \<subseteq> cs"
+  by (simp add: ubDom_rep_eq ubRestrict_insert)
+
+(* the dom of the bundle after restrict its channel is the conjunction of dom ub and first argument*)
+lemma ubRestrict_dom2 [simp]: "ubDom\<cdot>(ubRestrict cs\<cdot>ub) = ubDom\<cdot>ub \<inter> cs"
+  by (metis dom_restrict ubDom_insert ubDom_rep_eq ubRestrict_insert ubRestrict_well)
+
+
+(* applying 2 times ubRestriction on a ubundle is eq the application of the function with the union of both channel set as argument  *)
+lemma ubRestrict_twice [simp]: "ubRestrict cs2\<cdot>(ubRestrict cs1\<cdot>ub) = ubRestrict (cs1\<inter>cs2)\<cdot>ub"
+  by (metis restrict_restrict ubRestrict_insert ubRestrict_rep_eq ubRestrict_well)
+
+(* the element in the channel after restriction is equal the unrestrict bundle *)
+lemma ubGetCh_restrict [simp]: assumes "c \<in> cs"
+  shows "ubGetCh c\<cdot>(ubRestrict cs\<cdot>ub) = ubGetCh c\<cdot>ub"
+  by (metis (no_types, lifting) Abs_cfun_inverse2 assms restrict_in ubGetCh_def ubGetCh_cont ubGetCh_rep_eq ubRestrict_insert ubRestrict_well)
+
+(* the bundles after applying ubRestrict have the same below relation like its second  *)
+lemma ubRestrict_belowI1: assumes "(a \<sqsubseteq> b)"
+  shows "ubRestrict cs\<cdot>a \<sqsubseteq> ubRestrict cs\<cdot>b"
+  using assms monofun_cfun_arg by auto
+
+(* if an empty channel set is the first argument, then ubRestrict return the ubLeast with empty channel set  *)
+lemma ubRestrict_least [simp]: "ubRestrict {}\<cdot>ub = ubLeast {}"
+  by (metis Rep_ubundle_inverse empty_iff empty_subsetI optionleast_dom part_eq subset_antisym ubLeast_optionLeast_eq ubDom_insert ubRestrict_dom)
+
+(* if the first argument disjoint with the domain of the bundle then the function return ubLeast with an empty channel set *)
+lemma ubRestrict_least2[simp]: assumes "cs \<inter> ubDom\<cdot>ub = {}" 
+  shows "ubRestrict cs\<cdot>ub = ubLeast {}"
+  by (metis Int_commute Int_empty_right assms dom_restrict ex_in_conv part_eq ubDom_insert ubRestrict_insert ubRestrict_least)
+
+
+lemma ubRestrict_id [simp]: assumes "ubDom\<cdot>ub \<subseteq> cs" shows "ubRestrict cs\<cdot>ub = ub"
+  by (metis (mono_tags, lifting) assms contra_subsetD inf.absorb_iff1 ubGetChI ubGetCh_restrict ubRestrict_dom2)
+
+
+
+  subsection \<open>ubLen\<close>
+(* ubLen *) 
+  thm ubLen_def
+
+
+  subsection \<open>ubShift\<close>
 (* ubShift *) 
+  thm ubShift_def
+(*
+definition ubShift :: "('a \<Rightarrow> 'b) \<Rightarrow> 'a ubundle \<Rightarrow> 'b ubundle" where
+"ubShift f sb = Abs_ubundle (\<lambda>c. ((c\<in>ubDom\<cdot>sb) \<leadsto> f (ubGetCh c\<cdot>sb)))"
+*)
+
   
 (* ubUnion *)
 
